Flapjack.lean
@@ -43,6 +43,7 @@ import Flapjack.LoopSemantics
 import Flapjack.Word
 import Flapjack.Stack
 import Flapjack.StackAlloc
+import Flapjack.StackAlloc.Runtime
 import Flapjack.StackRemove
 import Flapjack.Lab
 import Flapjack.RiscV.Lab
